CompileModule with just one nagging admit, which probably indicates a code bug

platform/Depl/CompileModule.v
@@ -33,13 +33,14 @@ Record function := {
 Fixpoint formals (V : vals) (xs : list pr_var) (fE : fo_env) : fo_env :=
   match xs with
     | nil => fE
-    | x :: xs => fo_set (formals V xs fE) x (Dyn (sel V x))
+    | x :: xs => fo_set (formals V xs fE) (x ++ "0")%string (Dyn (sel V x))
   end.
 
 (** Generic top-level function spec (see [Compile.precond] for comments) *)
 Definition precond (frmls lcls : list pr_var) (pre post : pred) (inBody : bool) : assert :=
-  (PRE[V] mallocHeap 0 * predD pre (formals V frmls fo_empty)
-   POST[R] mallocHeap 0 * predD post (fo_set (formals V frmls fo_empty) "result" (Dyn R)))
+  (Al fE,
+    PRE[V] mallocHeap 0 * predD pre (formals V frmls fE)
+    POST[R] mallocHeap 0 * predD post (fo_set (formals V frmls fE) "result" (Dyn R)))
   false (fun w => w) (if inBody then frmls ++ lcls else frmls) (if inBody then 0 else length lcls).
 
 (** A default function, for when things go horribly wrong *)
@@ -69,8 +70,8 @@ Definition compileFunction (f : function) : Programming.function :=
           Structured nil (fun im mn _ => Structured.Assert_ im mn
             (precond (Formals f) (Locals f) (Precondition f) (Postcondition f) true)));;
         (fun _ _ => Stmt (map (fun s => s ++ "0")%string xs ++ SpecVars f)
-          bvs bvs' xs (vars0 xs)
-          (Precondition f) (Postcondition f) (Body f) (Formals f ++ Locals f) 0))%SP
+          bvs bvs' xs (vars0 (Formals f))
+          (Precondition f) (Postcondition f) (Body f) xs 0))%SP
     |}
     | _, _ => function0 (Name f)
   end.
@@ -93,6 +94,23 @@ Section NoDup_dec.
   Defined.
 End NoDup_dec.
 
+(** Does a list of variables include any ending in "0"?
+  * We're using that convention for our automatically generated variables,
+  * so it's a no-no for the programmer to use it. *)
+
+Fixpoint anyZero (x : fo_var) : bool :=
+  match x with
+    | "" => false
+    | "0" => true
+    | String _ x' => anyZero x'
+  end.
+
+Fixpoint anyZeros (xs : list fo_var) : bool :=
+  match xs with
+    | nil => false
+    | x :: xs' => anyZero x || anyZeros xs'
+  end.
+
 (** A computable syntactic well-formedness check... *)
 Definition functionWf (f : function) : bool :=
   let xs := Formals f ++ Locals f in
@@ -102,6 +120,8 @@ Definition functionWf (f : function) : bool :=
   else if in_dec string_dec "result" fvs
     then false
   else if (if NoDup_dec _ string_dec xs then false else true)
+    then false
+  else if anyZeros (SpecVars f)
     then false
   else match boundVars (Precondition f), boundVars (Postcondition f) with
          | Some bvs, Some bvs' =>
@@ -116,7 +136,8 @@ Definition functionVc (f : function) : list Prop :=
   let xs := Formals f ++ Locals f in
   let fvs := map (fun s => s ++ "0")%string xs ++ SpecVars f in
     stmtV xs (Body f)
-    :: stmtD (normalize (Precondition f)) (normalize (Postcondition f)) fvs (vars0 xs) (Body f) (fun _ => False)
+    :: stmtD (normalize (Precondition f))
+    (normalize (Postcondition f)) fvs (vars0 (Formals f)) (Body f) (fun _ => False)
     :: wellScoped fvs (Precondition f)
     :: wellScoped ("result" :: fvs) (Postcondition f)
     :: predExt (Precondition f)
@@ -171,6 +192,17 @@ Proof.
   eapply normalize_sound_bwd; eauto.
 Qed.
 
+Lemma weaken_predD : forall p xs fE fE',
+  wellScoped xs p
+  -> (forall x, In x xs -> fE x = fE' x)
+  -> predD p fE ===> predD p fE'.
+Proof.
+  intros.
+  change (predD p fE) with (SubstsH (SNil _ _) (predD p fE)).
+  change (predD p fE') with (SubstsH (SNil _ _) (predD p fE')).
+  eapply weaken_predD; eauto.
+Qed.
+
 (** Relate the above definitions to what [StructuredModule] wants. *)
 Theorem makeVcs_correct : forall mn fs0 fs, functionsWf fs = true
   -> vcs (makeVcs fs)
@@ -186,7 +218,13 @@ Proof.
   apply andb_prop in H; intuition.
   unfold functionWf in H1.
   unfold compileFunction at 1.
+
   repeat match goal with
+           | [ H : context[if anyZeros ?X then _ else _] |- _ ] =>
+             case_eq (anyZeros X); intros;
+               match goal with
+                 | [ H' : _ = _ |- _ ] => rewrite H' in *
+               end; try discriminate
            | [ H : context[if (if ?E then _ else _) then _ else _] |- _ ] => destruct E; try discriminate
            | [ H : context[if ?E then _ else _] |- _ ] => destruct E; try discriminate
            | [ H : context[match ?E with None => _ | _ => _ end] |- _ ] => case_eq E; intros;
@@ -201,22 +239,104 @@ Proof.
   post; clear_fancier.
   assert (In "rp" ("rp" :: Formals a)) by (simpl; tauto).
   assert (~In "rp" (Formals a)) by (intro; apply n0; eauto using in_or_app).
-  change (sel x0) with x0 in *.
+  change (sel x1) with x1 in *.
   unfold lvalIn, regInL in *; simpl in H1.
   change (LvMem (Indir Sp (natToW O))) with (LvMem (Indir Sp (variablePosition ("rp" :: Formals a) "rp"))) in *.
   evaluate auto_ext.
 
-  post; clear_fancier.
-  change (locals ("rp" :: Formals a) x1 (length (Locals a)) (Regs x Sp))
-    with (locals_in ("rp" :: Formals a) x1 (length (Locals a)) (Regs x Sp)
+  post.
+  assert (forall x4 x v, In x (map (fun s : string => (s ++ "0")%string) (Formals a ++ Locals a) ++ SpecVars a)
+    -> formals x2 (Formals a) x0 x
+    = formals (upd (merge x2 x4 ("rp" :: Formals a)) "rp" v)
+    (Formals a) x0 x).
+  intros.
+  apply in_app_or in H; intuition idtac.
+  apply in_map_iff in H18; destruct H18; intuition subst.
+
+  Lemma append0_invert : forall x y,
+    (x ++ "0" = y ++ "0")%string
+    -> x = y.
+  Proof.
+    induction x; destruct y; simpl in *; intuition.
+    destruct y; discriminate.
+    destruct x; discriminate.
+    injection H; clear H; intros; subst.
+    f_equal; auto.
+  Qed.
+
+  Lemma formals_switch : forall V V' x xs fE,
+    (In x xs -> sel V x = sel V' x)
+    -> formals V xs fE (x ++ "0")%string = formals V' xs fE (x ++ "0")%string.
+  Proof.
+    induction xs; simpl; intuition.
+    unfold fo_set.
+    destruct (string_dec (x ++ "0")%string (a ++ "0")%string); subst; auto.
+    apply append0_invert in e; subst.
+    f_equal; auto.
+  Qed.
+
+  apply formals_switch.
+  apply in_app_or in H19; intuition idtac.
+  rewrite sel_upd_ne.
+  symmetry; apply sel_merge.
+  simpl; tauto.
+  intro; subst.
+  eauto using in_or_app.
+
+  Lemma NoDup_unapp : forall A (ls2 ls1 : list A),
+    NoDup (ls1 ++ ls2)
+    -> forall x, In x ls1 -> In x ls2 -> False.
+  Proof.
+    induction ls1; inversion 1; simpl; intuition (subst; eauto using in_or_app).
+  Qed.
+
+  exfalso; eauto using NoDup_unapp.
+  
+  Lemma anyZero_duh : forall s, anyZero (s ++ "0")%string = true.
+  Proof.
+    induction s; simpl; intuition.
+    destruct a.
+    rewrite IHs.
+    repeat match goal with
+             | [ |- (if ?E then _ else _) = _ ] => destruct E; auto
+           end.
+  Qed.
+
+  Lemma formals_irrel : forall V V' x xs fE,
+    anyZero x = false
+    -> formals V xs fE x = formals V' xs fE x.
+  Proof.
+    induction xs; simpl; intuition.
+    unfold fo_set.
+    destruct (string_dec x (a ++ "0")%string); subst; auto.
+    rewrite anyZero_duh in H; discriminate.
+  Qed.
+
+  Lemma anyZeros_correct : forall x xs, anyZeros xs = false
+    -> In x xs
+    -> anyZero x = false.
+  Proof.
+    induction xs; simpl; intuition subst.
+
+    apply orb_false_iff in H; intuition.
+    apply orb_false_iff in H; intuition.
+  Qed.
+
+  eauto using formals_irrel, anyZeros_correct.
+
+  generalize dependent (map (fun s : string => (s ++ "0")%string) (Formals a ++ Locals a) ++ SpecVars a); intros.
+  clear_fancier.
+  clear H8.
+  change (locals ("rp" :: Formals a) x2 (length (Locals a)) (Regs x Sp))
+    with (locals_in ("rp" :: Formals a) x2 (length (Locals a)) (Regs x Sp)
       (Locals a) ("rp" :: Formals a ++ Locals a) 0) in *.
   assert (ok_in ("rp" :: Formals a) (length (Locals a))
     (Locals a) ("rp" :: Formals a ++ Locals a) 0).
   repeat split; unfold pr_var; auto; try omega.
   simpl; constructor; auto.
   assert (In "rp" ("rp" :: Formals a ++ Locals a)) by (simpl; tauto).
-  change (sel x1) with x1 in *.
-  unfold lvalIn, regInL in *; simpl in H13.
+  change (sel x2) with x2 in *.
+  unfold lvalIn, regInL in *; simpl in H14.
   change (LvMem (Indir Sp (natToW O))) with (LvMem (Indir Sp (variablePosition ("rp" :: Formals a ++ Locals a) "rp"))) in *.
   evaluate auto_ext.
   fold (@app pr_var) in *.
@@ -224,35 +344,70 @@ Proof.
   rewrite sel_eta.
   step auto_ext.
   etransitivity; [ apply himp_star_comm | ]; apply himp_star_frame; try reflexivity.
-  admit. (* Interaction of [formals] and [merge] *)
-  step auto_ext.
+  eapply weaken_predD; eauto.
+  eauto.
   step auto_ext.
   descend; step auto_ext.
-  instantiate (1 := x5).
-  change (locals ("rp" :: Formals a) x5 (Datatypes.length (Locals a)) (Regs x Sp))
-    with (locals_out ("rp" :: Formals a) x5 (Datatypes.length (Locals a)) (Regs x Sp)
+  instantiate (1 := x6).
+  change (locals ("rp" :: Formals a) x6 (Datatypes.length (Locals a)) (Regs x Sp))
+    with (locals_out ("rp" :: Formals a) x6 (Datatypes.length (Locals a)) (Regs x Sp)
       (Locals a) ("rp" :: Formals a ++ Locals a) 0).
   assert (ok_out ("rp" :: Formals a) (Datatypes.length (Locals a))
     (Locals a) ("rp" :: Formals a ++ Locals a) 0).
   repeat split; unfold pr_var; auto; try omega.
   rewrite sel_eta.
   descend; step auto_ext.
-  admit. (* Interaction of [formals] and [merge] *)
+  eapply weaken_predD; eauto.
+  simpl; intuition (subst; eauto).
+  unfold fo_set.
+  destruct (string_dec x6 "result"); subst; auto.
+  symmetry; auto.
+
 
   post.
   generalize dependent (map (fun s : string => (s ++ "0")%string) (Formals a ++ Locals a) ++ SpecVars a); intros.
   clear_fancier.
-  clear H7.
+  clear H8.
   descend.
   repeat rewrite sel_eta in *.
   step auto_ext.
   fold (@app pr_var).
   Focus 2.
   apply himp_star_frame; try reflexivity.
-
   eapply normalize_sound_fwd; eauto using notsInList_true.
-  admit. (* [vars_ok] with [formals] *)
-  replace (sel x0 "rp") with (st#Rp) by admit.
+
+  Lemma formals_grab : forall V x xs fE,
+    In x xs
+    -> formals V xs fE (x ++ "0")%string = Dyn (sel V x).
+  Proof.
+    induction xs; simpl; intuition (subst; eauto).
+    unfold fo_set.
+    destruct (string_dec (x ++ "0")%string (x ++ "0")%string); subst; congruence.
+    unfold fo_set.
+    destruct (string_dec (x ++ "0")%string (a ++ "0")%string); subst; auto.
+    apply append0_invert in e; subst.
+    auto.
+  Qed.
+
+  Lemma vars_ok_formals : forall V xs fE,
+    vars_ok (formals V xs fE) V (vars0 xs).
+  Proof.
+    unfold vars_ok, vars0; induction xs; simpl; intuition.
+
+    destruct (string_dec a x); subst.
+    injection H; clear H; intros; subst; simpl.
+    unfold fo_set.
+    destruct (string_dec (x ++ "0") (x ++ "0")); tauto.
+    destruct (in_dec string_dec x xs); try discriminate.
+    injection H; clear H; intros; subst; simpl.
+    unfold fo_set.
+    destruct (string_dec (x ++ "0") (a ++ "0")).
+    apply append0_invert in e; congruence.
+    auto using formals_grab.
+  Qed.
+
+  apply vars_ok_formals.
+  replace (sel x1 "rp") with (st#Rp) by admit.
   step auto_ext.
   step auto_ext.
   descend; step auto_ext.
@@ -264,20 +419,16 @@ Proof.
   hnf; auto.
 
   unfold vars0 in *.
-  destruct (in_dec string_dec x (Formals a ++ Locals a)); auto; congruence.
-
-  unfold vars0 in *.
-  destruct (in_dec string_dec x (Formals a ++ Locals a)); try discriminate.
-  inversion_clear H.
-  simpl.
+  destruct (in_dec string_dec x (Formals a)); auto; try congruence.
+  injection H; clear H; intros; subst; simpl.
   apply H1.
   apply in_or_app; left.
-  apply in_map_iff; eauto.
+  apply in_map_iff; eauto using in_or_app.
 
   eauto using notsInList_true.
-  eapply notsInList_true in H6; eauto.
-  subst; simpl; tauto.
-  eapply notsInList_true in H6; eauto.
+  subst.
+  eapply notsInList_true in H7; intuition; auto.
+  eapply notsInList_true in H7; eauto.
   subst; simpl; tauto.
 Qed.
 
